theories/language/wp_link.v
@@ -189,6 +189,9 @@ Definition program_fulfills
   (Tin : program_specification) (p : mixin_prog (func Λ)) (Tshould : program_specification) : iProp Σ := 
   ∀ s vv Φ, Tshould s vv Φ -∗ ⌜p !! s <> None⌝ ∗ WP (of_class _ (ExprCall s vv)) @ (mkPe p Tin); ⊤ {{v, Φ v}}.
 
+Definition env_fulfills
+  (p:prog_environ) (Tshould : program_specification) := program_fulfills (p.(T)) (p.(prog)) Tshould.
+
 Notation "Tin '|-' p '::' Tshould" := (program_fulfills Tin p Tshould) (at level 25, p, Tshould at level 26) : bi_scope.
 
 Definition spec_union (p1 p2 : program_specification) : program_specification := 
@@ -239,211 +242,218 @@ Proof.
   - eapply head_step_no_call; done. 
 Qed.
 
-Lemma link_progs T1 T2 T3 (p1 p2 : gmap string (Λ.(func))) :
-    ⌜dom p1 ## dom p2⌝
- -∗ □(∀ s vv Φ, T3 s vv Φ -∗ ⌜s ∉ dom p1⌝ ∗ ⌜s ∉ dom p2⌝)
- -∗ □(spec_union T2 T3 |- p1 :: T1)
- -∗ □(spec_union T1 T3 |- p2 :: T2)
- -∗ T3 |- (union_with (fun a b => None) p1 p2) :: (spec_union T1 T2).
-Proof.
-  iIntros (Hdis) "#HT3 #Hp1 #Hp2".
-  iAssert (∀ e Φ,
+Definition can_link T1 T2 T3 Tres (p1 p2 p3 : gmap string (Λ.(func))) :iProp Σ := 
+   ⌜dom p1 ## dom p2⌝
+ ∗ □(∀ s vv Φ, T3 s vv Φ -∗ ⌜s ∉ dom p1⌝ ∗ ⌜s ∉ dom p2⌝)
+ ∗ □(∀ s vv Φ, Tres s vv Φ -∗ (spec_union T1 T2) s vv Φ)
+ ∗ □(spec_union T2 T3 |- p1 :: T1)
+ ∗ □(spec_union T1 T3 |- p2 :: T2)
+ ∗ ⌜p3 = (union_with (λ _ _ : func Λ, None) p1 p2)⌝.
+
+Lemma wp_link_execs T1 T2 T3 Tres (p1 p2 p3 : gmap string (Λ.(func))) :
+  can_link T1 T2 T3 Tres p1 p2 p3
+ -∗ ∀ e Φ,
     WP e @ mkPe p1 (spec_union T2 T3); ⊤ {{ v, Φ v }} ∨ WP e @ mkPe p2 (spec_union T1 T3); ⊤ {{ v, Φ v }} -∗
-    WP e @ mkPe (union_with (λ _ _ : func Λ, None) p1 p2) (T3); ⊤ {{ v, Φ v }}
-    )%I as "Hen".
-  + iLöb as "IHe". iIntros (e Φ).
-    rewrite !wp_unfold /wp_pre /=.
-    iIntros "[H|H] %σ %ns Hσ".
-    - iSpecialize ("H" $! σ ns with "Hσ").
-      iMod "H".
-      iDestruct "H" as "[(%x & -> & Hσ & H)|[(%s' & %vv' & %K & %HeqK & %H2 & >(%Ξ & Hσ & [HT|HT] & H3))|(%HH & H3)]]".
-      * iModIntro. iLeft. iExists _. iFrame. iPureIntro. done.
-      * destruct (p2 !! s') as [v|] eqn:Heqp2.
-        ++ iRight. iRight.
-           iPoseProof ("Hp2" $! _ _ _ with "HT") as "(%HNone & HT)".
-           rewrite wp_unfold /wp_pre /=.
-           iSpecialize ("HT" $! σ ns with "Hσ").
-           iMod "HT" as "[(%x & %Heqx & Hσ & H)|[(%s'2 & %vv'2 & %K'2 & %HeqK2 & %H''2 & >(%Ξ' & Hσ & HT' & H3'))|(%HH2&H3')]]".
-           -- exfalso. apply of_class_inj in Heqx. congruence.
-           -- exfalso. assert (K'2 = empty_ectx) as ->. 
-              2: { rewrite fill_empty in HeqK2. apply of_class_inj in HeqK2. assert (s'2 = s') as -> by congruence; congruence. }
-              destruct (fill_class K'2 (of_class Λ (ExprCall s'2 vv'2))) as [H1|[x Hx]].
-              { eexists. rewrite <- HeqK2. by rewrite to_of_class. }
-              { done. }
-              { exfalso. unfold to_val in Hx. rewrite to_of_class in Hx; congruence. }
-           -- destruct HH2 as (e' & σ' & (KK & e1' & e2' & Heq2 & -> & Hstep)%prim_step_inv).
-              destruct (fill_class KK e1') as [->|[x Hx]].
-              { eexists. rewrite <- Heq2. by rewrite to_of_class. }
-              2: { apply val_head_stuck in Hstep. congruence. }
-              rewrite ! fill_empty in Heq2. subst e1'.
-              apply call_head_step in Hstep.
-              destruct Hstep as (Fn & Heqp2' & He2' & -> & _ ).
-              iModIntro. iSplit; first iPureIntro.
-              { do 2 eexists. rewrite HeqK. econstructor; first done. 1:done.
-                apply call_head_step. exists Fn. repeat split; try done.
-                rewrite lookup_union_with. rewrite Heqp2'. rewrite H2. done. }
-              subst e. iIntros (? ? (e'2 & -> & (Fn3 & Heqp3' & He3' & -> & _ )%call_head_step)%head_reducible_prim_step_ctx).
-              2: { do 3 eexists.
-                   apply call_head_step. exists Fn. repeat split; try done.
-                   rewrite lookup_union_with. rewrite Heqp2'. rewrite H2. done. }
-              rewrite lookup_union_with in Heqp3'. rewrite Heqp2' in Heqp3'. rewrite H2 in Heqp3'.
-              cbn in Heqp3'. iSpecialize ("H3'" $! σ e2').
-              assert (prim_step p2 (of_class Λ (ExprCall s' vv')) σ e2' σ []) as Hstep2.
-              { apply head_prim_step. apply call_head_step. eexists; repeat split; done. }
-              iSpecialize ("H3'" $! Hstep2). iMod "H3'". iModIntro. iNext.
-              iMod "H3'" as "(? & H3')". iModIntro. iFrame.
-              iApply wp_bind. iApply (wp_wand with "[H3']").
-              { iApply "IHe"; iRight. assert (e'2 = e2') as -> by congruence. iApply "H3'". }
-              iIntros (r) "Hr". iSpecialize ("H3" $! r with "Hr"). iApply "IHe". iLeft. done.
-        ++ iRight. iLeft. iModIntro.
-           rewrite HeqK. do 3 iExists _. iSplitR; first done.
-           iSplitR.
-           { iPureIntro. rewrite lookup_union_with. rewrite H2. rewrite Heqp2. done. }
-           iDestruct ("Hp2" with "HT") as "(%HNone2 & _)". congruence.
-      * iRight. iLeft. iModIntro. do 3 iExists _; iSplitR; first done.
-        rewrite lookup_union_with. rewrite H2. destruct (p2!!s') eqn:Heq.
-        1: { iDestruct ("HT3" with "HT") as "(%Hne1 & %Hne2)".
-             exfalso. apply Hne2. apply elem_of_dom. by eexists. }
-        cbn. iSplitR; first done. iModIntro. iExists Ξ. iFrame. iNext.
-        iIntros (r) "Hr". iSpecialize ("H3" with "Hr"). iApply "IHe". iLeft. done.
-      * iModIntro. iRight. iRight.
-        iSplitR.
-        { iPureIntro. eapply reducible_no_threads_mono; last done.
-          intros k. rewrite lookup_union_with. destruct (p1 !! k) as [f1|] eqn:Heq1;
-          destruct (p2 !! k) as [f2|] eqn:Heq2.
-          2-4: done. 
-          cbn. apply elem_of_disjoint in Hdis. eapply Hdis; apply elem_of_dom; eexists; done. }
-        iIntros (σ' e' Hstep%prim_step_inv).
-        iSpecialize ("H3" $! σ' e').
-        destruct Hstep as (K & e1' & e2' & -> & -> & H).
-        assert (prim_step p1 (fill K e1') σ (fill K e2') σ' []) as Hstep.
-        { econstructor. 1-2:done. destruct (to_class e1') as [[]|] eqn:Heq.
-          - exfalso. eapply val_head_step. apply of_to_class in Heq. erewrite Heq. done.
-          - apply of_to_class in Heq. subst e1'.
-            destruct HH as (? & σ'2 & (e2'' & -> & (K2 & eK1 & eK2 & Heq1 & -> & HHstep)%prim_step_inv)%fill_step_inv).
-            2: unfold to_val; by rewrite to_of_class.
-            assert (K2 = empty_ectx) as ->.
-            1: { destruct (fill_class' K2 eK1) as [|[vv Hvv]].
-                 1: eexists; rewrite <- Heq1; by rewrite to_of_class.
-                 1: done.
-                 exfalso. apply of_to_class in Hvv. subst eK1. eapply val_head_step. done. }
-            rewrite fill_empty in Heq1. subst eK1. apply call_head_step in H, HHstep.
-            destruct H as (FN1 & HFN1 &Happy1 & -> & _).
-            destruct HHstep as (FN2 & HFN2 &Happy2 & -> & _).
-            rewrite lookup_union_with in HFN1. rewrite HFN2 in HFN1. destruct (p2 !! fn_name); cbn in *; try congruence.
-            apply call_head_step. exists FN2. repeat split; try congruence.
-          - by eapply head_step_no_call. }
-        iDestruct ("H3" $! Hstep) as ">H3". iModIntro. iNext.
-        iMod "H3" as "(Hσ & HWP)". iModIntro. iFrame. iApply "IHe". by iLeft.
+    WP e @ mkPe p3 (T3); ⊤ {{ v, Φ v }}.
+Proof.
+  iIntros "(%Hdis & #HT3 & _ & #Hp1 & #Hp2 & ->)".
+  iLöb as "IHe". iIntros (e Φ).
+  rewrite !wp_unfold /wp_pre /=.
+  iIntros "[H|H] %σ %ns Hσ".
+  - iSpecialize ("H" $! σ ns with "Hσ").
+    iMod "H".
+    iDestruct "H" as "[(%x & -> & Hσ & H)|[(%s' & %vv' & %K & %HeqK & %H2 & >(%Ξ & Hσ & [HT|HT] & H3))|(%HH & H3)]]".
+    * iModIntro. iLeft. iExists _. iFrame. iPureIntro. done.
+    * destruct (p2 !! s') as [v|] eqn:Heqp2.
+      ++ iRight. iRight.
+         iPoseProof ("Hp2" $! _ _ _ with "HT") as "(%HNone & HT)".
+         rewrite wp_unfold /wp_pre /=.
+         iSpecialize ("HT" $! σ ns with "Hσ").
+         iMod "HT" as "[(%x & %Heqx & Hσ & H)|[(%s'2 & %vv'2 & %K'2 & %HeqK2 & %H''2 & >(%Ξ' & Hσ & HT' & H3'))|(%HH2&H3')]]".
+         -- exfalso. apply of_class_inj in Heqx. congruence.
+         -- exfalso. assert (K'2 = empty_ectx) as ->. 
+            2: { rewrite fill_empty in HeqK2. apply of_class_inj in HeqK2. assert (s'2 = s') as -> by congruence; congruence. }
+            destruct (fill_class K'2 (of_class Λ (ExprCall s'2 vv'2))) as [H1|[x Hx]].
+            { eexists. rewrite <- HeqK2. by rewrite to_of_class. }
+            { done. }
+            { exfalso. unfold to_val in Hx. rewrite to_of_class in Hx; congruence. }
+         -- destruct HH2 as (e' & σ' & (KK & e1' & e2' & Heq2 & -> & Hstep)%prim_step_inv).
+            destruct (fill_class KK e1') as [->|[x Hx]].
+            { eexists. rewrite <- Heq2. by rewrite to_of_class. }
+            2: { apply val_head_stuck in Hstep. congruence. }
+            rewrite ! fill_empty in Heq2. subst e1'.
+            apply call_head_step in Hstep.
+            destruct Hstep as (Fn & Heqp2' & He2' & -> & _ ).
+            iModIntro. iSplit; first iPureIntro.
+            { do 2 eexists. rewrite HeqK. econstructor; first done. 1:done.
+              apply call_head_step. exists Fn. repeat split; try done.
+              rewrite lookup_union_with. rewrite Heqp2'. rewrite H2. done. }
+            subst e. iIntros (? ? (e'2 & -> & (Fn3 & Heqp3' & He3' & -> & _ )%call_head_step)%head_reducible_prim_step_ctx).
+            2: { do 3 eexists.
+                 apply call_head_step. exists Fn. repeat split; try done.
+                 rewrite lookup_union_with. rewrite Heqp2'. rewrite H2. done. }
+            rewrite lookup_union_with in Heqp3'. rewrite Heqp2' in Heqp3'. rewrite H2 in Heqp3'.
+            cbn in Heqp3'. iSpecialize ("H3'" $! σ e2').
+            assert (prim_step p2 (of_class Λ (ExprCall s' vv')) σ e2' σ []) as Hstep2.
+            { apply head_prim_step. apply call_head_step. eexists; repeat split; done. }
+            iSpecialize ("H3'" $! Hstep2). iMod "H3'". iModIntro. iNext.
+            iMod "H3'" as "(? & H3')". iModIntro. iFrame.
+            iApply wp_bind. iApply (wp_wand with "[H3']").
+            { iApply "IHe"; iRight. assert (e'2 = e2') as -> by congruence. iApply "H3'". }
+            iIntros (r) "Hr". iSpecialize ("H3" $! r with "Hr"). iApply "IHe". iLeft. done.
+      ++ iRight. iLeft. iModIntro.
+         rewrite HeqK. do 3 iExists _. iSplitR; first done.
+         iSplitR.
+         { iPureIntro. rewrite lookup_union_with. rewrite H2. rewrite Heqp2. done. }
+         iDestruct ("Hp2" with "HT") as "(%HNone2 & _)". congruence.
+    * iRight. iLeft. iModIntro. do 3 iExists _; iSplitR; first done.
+      rewrite lookup_union_with. rewrite H2. destruct (p2!!s') eqn:Heq.
+      1: { iDestruct ("HT3" with "HT") as "(%Hne1 & %Hne2)".
+           exfalso. apply Hne2. apply elem_of_dom. by eexists. }
+      cbn. iSplitR; first done. iModIntro. iExists Ξ. iFrame. iNext.
+      iIntros (r) "Hr". iSpecialize ("H3" with "Hr"). iApply "IHe". iLeft. done.
+    * iModIntro. iRight. iRight.
+      iSplitR.
+      { iPureIntro. eapply reducible_no_threads_mono; last done.
+        intros k. rewrite lookup_union_with. destruct (p1 !! k) as [f1|] eqn:Heq1;
+        destruct (p2 !! k) as [f2|] eqn:Heq2.
+        2-4: done. 
+        cbn. apply elem_of_disjoint in Hdis. eapply Hdis; apply elem_of_dom; eexists; done. }
+      iIntros (σ' e' Hstep%prim_step_inv).
+      iSpecialize ("H3" $! σ' e').
+      destruct Hstep as (K & e1' & e2' & -> & -> & H).
+      assert (prim_step p1 (fill K e1') σ (fill K e2') σ' []) as Hstep.
+      { econstructor. 1-2:done. destruct (to_class e1') as [[]|] eqn:Heq.
+        - exfalso. eapply val_head_step. apply of_to_class in Heq. erewrite Heq. done.
+        - apply of_to_class in Heq. subst e1'.
+          destruct HH as (? & σ'2 & (e2'' & -> & (K2 & eK1 & eK2 & Heq1 & -> & HHstep)%prim_step_inv)%fill_step_inv).
+          2: unfold to_val; by rewrite to_of_class.
+          assert (K2 = empty_ectx) as ->.
+          1: { destruct (fill_class' K2 eK1) as [|[vv Hvv]].
+               1: eexists; rewrite <- Heq1; by rewrite to_of_class.
+               1: done.
+               exfalso. apply of_to_class in Hvv. subst eK1. eapply val_head_step. done. }
+          rewrite fill_empty in Heq1. subst eK1. apply call_head_step in H, HHstep.
+          destruct H as (FN1 & HFN1 &Happy1 & -> & _).
+          destruct HHstep as (FN2 & HFN2 &Happy2 & -> & _).
+          rewrite lookup_union_with in HFN1. rewrite HFN2 in HFN1. destruct (p2 !! fn_name); cbn in *; try congruence.
+          apply call_head_step. exists FN2. repeat split; try congruence.
+        - by eapply head_step_no_call. }
+      iDestruct ("H3" $! Hstep) as ">H3". iModIntro. iNext.
+      iMod "H3" as "(Hσ & HWP)". iModIntro. iFrame. iApply "IHe". by iLeft.
 
 
 
 
-    - iSpecialize ("H" $! σ ns with "Hσ").
-      iMod "H".
-      iDestruct "H" as "[(%x & -> & Hσ & H)|[(%s' & %vv' & %K & %HeqK & %H2 & >(%Ξ & Hσ & [HT|HT] & H3))|(%HH & H3)]]".
-      * iModIntro. iLeft. iExists _. iFrame. iPureIntro. done.
-      * destruct (p1 !! s') as [v|] eqn:Heqp2.
-        ++ iRight. iRight.
-           iPoseProof ("Hp1" $! _ _ _ with "HT") as "(_ & HT)".
-           rewrite wp_unfold /wp_pre /=.
-           iSpecialize ("HT" $! σ ns with "Hσ").
-           iMod "HT" as "[(%x & %Heqx & Hσ & H)|[(%s'2 & %vv'2 & %K'2 & %HeqK2 & %H''2 & >(%Ξ' & Hσ & HT' & H3'))|(%HH2&H3')]]".
-           -- exfalso. apply of_class_inj in Heqx. congruence.
-           -- exfalso. assert (K'2 = empty_ectx) as ->. 
-              2: { rewrite fill_empty in HeqK2. apply of_class_inj in HeqK2. assert (s'2 = s') as -> by congruence; congruence. }
-              destruct (fill_class K'2 (of_class Λ (ExprCall s'2 vv'2))) as [H1|[x Hx]].
-              { eexists. rewrite <- HeqK2. by rewrite to_of_class. }
-              { done. }
-              { exfalso. unfold to_val in Hx. rewrite to_of_class in Hx; congruence. }
-           -- destruct HH2 as (e' & σ' & (KK & e1' & e2' & Heq2 & -> & Hstep)%prim_step_inv).
-              destruct (fill_class KK e1') as [->|[x Hx]].
-              { eexists. rewrite <- Heq2. by rewrite to_of_class. }
-              2: { apply val_head_stuck in Hstep. congruence. }
-              rewrite ! fill_empty in Heq2. subst e1'.
-              apply call_head_step in Hstep.
-              destruct Hstep as (Fn & Heqp2' & He2' & -> & _ ).
-              iModIntro. iSplit; first iPureIntro.
-              { do 2 eexists. rewrite HeqK. econstructor; first done. 1:done.
-                apply call_head_step. exists Fn. repeat split; try done.
-                rewrite lookup_union_with. rewrite Heqp2'. rewrite H2. done. }
-              subst e. iIntros (? ? (e'2 & -> & (Fn3 & Heqp3' & He3' & -> & _ )%call_head_step)%head_reducible_prim_step_ctx).
-              2: { do 3 eexists.
-                   apply call_head_step. exists Fn. repeat split; try done.
-                   rewrite lookup_union_with. rewrite Heqp2'. rewrite H2. done. }
-              rewrite lookup_union_with in Heqp3'. rewrite Heqp2' in Heqp3'. rewrite H2 in Heqp3'.
-              cbn in Heqp3'. iSpecialize ("H3'" $! σ e2').
-              assert (prim_step p1 (of_class Λ (ExprCall s' vv')) σ e2' σ []) as Hstep2.
-              { apply head_prim_step. apply call_head_step. eexists; repeat split; done. }
-              iSpecialize ("H3'" $! Hstep2). iMod "H3'". iModIntro. iNext.
-              iMod "H3'" as "(? & H3')". iModIntro. iFrame.
-              iApply wp_bind. iApply (wp_wand with "[H3']").
-              { iApply "IHe"; iLeft. assert (e'2 = e2') as -> by congruence. iApply "H3'". }
-              iIntros (r) "Hr". iSpecialize ("H3" $! r with "Hr"). iApply "IHe". iRight. done.
-        ++ iRight. iLeft. iModIntro.
-           rewrite HeqK. do 3 iExists _. iSplitR; first done.
-           iSplitR.
-           { iPureIntro. rewrite lookup_union_with. rewrite H2. rewrite Heqp2. done. }
-           iDestruct ("Hp1" with "HT") as "(%HNone2 & _)". congruence.
-      * iRight. iLeft. iModIntro. do 3 iExists _; iSplitR; first done.
-        rewrite lookup_union_with. rewrite H2. destruct (p1!!s') eqn:Heq.
-        1: { iDestruct ("HT3" with "HT") as "(%Hne1 & %Hne2)".
-             exfalso. apply Hne1. apply elem_of_dom. by eexists. }
-        cbn. iSplitR; first done. iModIntro. iExists Ξ. iFrame. iNext.
-        iIntros (r) "Hr". iSpecialize ("H3" with "Hr"). iApply "IHe". iRight. done.
-      * iModIntro. iRight. iRight.
-        iSplitR.
-        { iPureIntro. eapply reducible_no_threads_mono; last done.
-          intros k. rewrite lookup_union_with. destruct (p1 !! k) as [f1|] eqn:Heq1;
-          destruct (p2 !! k) as [f2|] eqn:Heq2.
-          2-4: done. 
-          cbn. apply elem_of_disjoint in Hdis. eapply Hdis; apply elem_of_dom; eexists; done. }
-        iIntros (σ' e' Hstep%prim_step_inv).
-        iSpecialize ("H3" $! σ' e').
-        destruct Hstep as (K & e1' & e2' & -> & -> & H).
-        assert (prim_step p2 (fill K e1') σ (fill K e2') σ' []) as Hstep.
-        { econstructor. 1-2:done. destruct (to_class e1') as [[]|] eqn:Heq.
-          - exfalso. eapply val_head_step. apply of_to_class in Heq. erewrite Heq. done.
-          - apply of_to_class in Heq. subst e1'.
-            destruct HH as (? & σ'2 & (e2'' & -> & (K2 & eK1 & eK2 & Heq1 & -> & HHstep)%prim_step_inv)%fill_step_inv).
-            2: unfold to_val; by rewrite to_of_class.
-            assert (K2 = empty_ectx) as ->.
-            1: { destruct (fill_class' K2 eK1) as [|[vv Hvv]].
-                 1: eexists; rewrite <- Heq1; by rewrite to_of_class.
-                 1: done.
-                 exfalso. apply of_to_class in Hvv. subst eK1. eapply val_head_step. done. }
-            rewrite fill_empty in Heq1. subst eK1. apply call_head_step in H, HHstep.
-            destruct H as (FN1 & HFN1 &Happy1 & -> & _).
-            destruct HHstep as (FN2 & HFN2 &Happy2 & -> & _).
-            rewrite lookup_union_with in HFN1. rewrite HFN2 in HFN1. destruct (p1 !! fn_name); cbn in *; try congruence.
-            apply call_head_step. exists FN2. repeat split; try congruence.
-          - by eapply head_step_no_call. }
-        iDestruct ("H3" $! Hstep) as ">H3". iModIntro. iNext.
-        iMod "H3" as "(Hσ & HWP)". iModIntro. iFrame. iApply "IHe". by iRight.
+  - iSpecialize ("H" $! σ ns with "Hσ").
+    iMod "H".
+    iDestruct "H" as "[(%x & -> & Hσ & H)|[(%s' & %vv' & %K & %HeqK & %H2 & >(%Ξ & Hσ & [HT|HT] & H3))|(%HH & H3)]]".
+    * iModIntro. iLeft. iExists _. iFrame. iPureIntro. done.
+    * destruct (p1 !! s') as [v|] eqn:Heqp2.
+      ++ iRight. iRight.
+         iPoseProof ("Hp1" $! _ _ _ with "HT") as "(_ & HT)".
+         rewrite wp_unfold /wp_pre /=.
+         iSpecialize ("HT" $! σ ns with "Hσ").
+         iMod "HT" as "[(%x & %Heqx & Hσ & H)|[(%s'2 & %vv'2 & %K'2 & %HeqK2 & %H''2 & >(%Ξ' & Hσ & HT' & H3'))|(%HH2&H3')]]".
+         -- exfalso. apply of_class_inj in Heqx. congruence.
+         -- exfalso. assert (K'2 = empty_ectx) as ->. 
+            2: { rewrite fill_empty in HeqK2. apply of_class_inj in HeqK2. assert (s'2 = s') as -> by congruence; congruence. }
+            destruct (fill_class K'2 (of_class Λ (ExprCall s'2 vv'2))) as [H1|[x Hx]].
+            { eexists. rewrite <- HeqK2. by rewrite to_of_class. }
+            { done. }
+            { exfalso. unfold to_val in Hx. rewrite to_of_class in Hx; congruence. }
+         -- destruct HH2 as (e' & σ' & (KK & e1' & e2' & Heq2 & -> & Hstep)%prim_step_inv).
+            destruct (fill_class KK e1') as [->|[x Hx]].
+            { eexists. rewrite <- Heq2. by rewrite to_of_class. }
+            2: { apply val_head_stuck in Hstep. congruence. }
+            rewrite ! fill_empty in Heq2. subst e1'.
+            apply call_head_step in Hstep.
+            destruct Hstep as (Fn & Heqp2' & He2' & -> & _ ).
+            iModIntro. iSplit; first iPureIntro.
+            { do 2 eexists. rewrite HeqK. econstructor; first done. 1:done.
+              apply call_head_step. exists Fn. repeat split; try done.
+              rewrite lookup_union_with. rewrite Heqp2'. rewrite H2. done. }
+            subst e. iIntros (? ? (e'2 & -> & (Fn3 & Heqp3' & He3' & -> & _ )%call_head_step)%head_reducible_prim_step_ctx).
+            2: { do 3 eexists.
+                 apply call_head_step. exists Fn. repeat split; try done.
+                 rewrite lookup_union_with. rewrite Heqp2'. rewrite H2. done. }
+            rewrite lookup_union_with in Heqp3'. rewrite Heqp2' in Heqp3'. rewrite H2 in Heqp3'.
+            cbn in Heqp3'. iSpecialize ("H3'" $! σ e2').
+            assert (prim_step p1 (of_class Λ (ExprCall s' vv')) σ e2' σ []) as Hstep2.
+            { apply head_prim_step. apply call_head_step. eexists; repeat split; done. }
+            iSpecialize ("H3'" $! Hstep2). iMod "H3'". iModIntro. iNext.
+            iMod "H3'" as "(? & H3')". iModIntro. iFrame.
+            iApply wp_bind. iApply (wp_wand with "[H3']").
+            { iApply "IHe"; iLeft. assert (e'2 = e2') as -> by congruence. iApply "H3'". }
+            iIntros (r) "Hr". iSpecialize ("H3" $! r with "Hr"). iApply "IHe". iRight. done.
+      ++ iRight. iLeft. iModIntro.
+         rewrite HeqK. do 3 iExists _. iSplitR; first done.
+         iSplitR.
+         { iPureIntro. rewrite lookup_union_with. rewrite H2. rewrite Heqp2. done. }
+         iDestruct ("Hp1" with "HT") as "(%HNone2 & _)". congruence.
+    * iRight. iLeft. iModIntro. do 3 iExists _; iSplitR; first done.
+      rewrite lookup_union_with. rewrite H2. destruct (p1!!s') eqn:Heq.
+      1: { iDestruct ("HT3" with "HT") as "(%Hne1 & %Hne2)".
+           exfalso. apply Hne1. apply elem_of_dom. by eexists. }
+      cbn. iSplitR; first done. iModIntro. iExists Ξ. iFrame. iNext.
+      iIntros (r) "Hr". iSpecialize ("H3" with "Hr"). iApply "IHe". iRight. done.
+    * iModIntro. iRight. iRight.
+      iSplitR.
+      { iPureIntro. eapply reducible_no_threads_mono; last done.
+        intros k. rewrite lookup_union_with. destruct (p1 !! k) as [f1|] eqn:Heq1;
+        destruct (p2 !! k) as [f2|] eqn:Heq2.
+        2-4: done. 
+        cbn. apply elem_of_disjoint in Hdis. eapply Hdis; apply elem_of_dom; eexists; done. }
+      iIntros (σ' e' Hstep%prim_step_inv).
+      iSpecialize ("H3" $! σ' e').
+      destruct Hstep as (K & e1' & e2' & -> & -> & H).
+      assert (prim_step p2 (fill K e1') σ (fill K e2') σ' []) as Hstep.
+      { econstructor. 1-2:done. destruct (to_class e1') as [[]|] eqn:Heq.
+        - exfalso. eapply val_head_step. apply of_to_class in Heq. erewrite Heq. done.
+        - apply of_to_class in Heq. subst e1'.
+          destruct HH as (? & σ'2 & (e2'' & -> & (K2 & eK1 & eK2 & Heq1 & -> & HHstep)%prim_step_inv)%fill_step_inv).
+          2: unfold to_val; by rewrite to_of_class.
+          assert (K2 = empty_ectx) as ->.
+          1: { destruct (fill_class' K2 eK1) as [|[vv Hvv]].
+               1: eexists; rewrite <- Heq1; by rewrite to_of_class.
+               1: done.
+               exfalso. apply of_to_class in Hvv. subst eK1. eapply val_head_step. done. }
+          rewrite fill_empty in Heq1. subst eK1. apply call_head_step in H, HHstep.
+          destruct H as (FN1 & HFN1 &Happy1 & -> & _).
+          destruct HHstep as (FN2 & HFN2 &Happy2 & -> & _).
+          rewrite lookup_union_with in HFN1. rewrite HFN2 in HFN1. destruct (p1 !! fn_name); cbn in *; try congruence.
+          apply call_head_step. exists FN2. repeat split; try congruence.
+        - by eapply head_step_no_call. }
+      iDestruct ("H3" $! Hstep) as ">H3". iModIntro. iNext.
+      iMod "H3" as "(Hσ & HWP)". iModIntro. iFrame. iApply "IHe". by iRight.
+Qed.
 
-
-  + iIntros (s vv Φ) "[H|H]".
-    - iDestruct ("Hp1" with "H") as "(%HNone & HH)".
-      destruct (p2 !! s) eqn:Heq.
-      * exfalso. pose proof (elem_of_disjoint (dom p1) (dom p2)) as [Hdis2 _].
-        destruct (p1 !! s) eqn:Heqq; try congruence.
-        eapply Hdis2; first done.
-        all: apply elem_of_dom; eexists; try done. 
-      * iSplitR.
-        -- iPureIntro. rewrite lookup_union_with. 
-           rewrite Heq. destruct (p1 !! s); cbn; congruence.
-        -- iApply "Hen". by iLeft.
-    - iDestruct ("Hp2" with "H") as "(%HNone & HH)".
-      destruct (p1 !! s) eqn:Heq.
-      * exfalso. pose proof (elem_of_disjoint (dom p1) (dom p2)) as [Hdis2 _].
-        destruct (p2 !! s) eqn:Heqq; try congruence.
-        eapply Hdis2; first done.
-        all: apply elem_of_dom; eexists; try done. 
-      * iSplitR.
-        -- iPureIntro. rewrite lookup_union_with. 
-           rewrite Heq. destruct (p2 !! s); cbn; congruence.
-        -- iApply "Hen". by iRight.
-
+Lemma wp_link_progs T1 T2 T3 Tres (p1 p2 p3 : gmap string (Λ.(func))) :
+    can_link T1 T2 T3 Tres p1 p2 p3
+ -∗ T3 |- p3 :: Tres.
+Proof.
+  iIntros "(%Hdis & #HT3 & #Hres & #Hp1 & #Hp2 & ->)".
+  iIntros (s vv Φ) "H". iDestruct ("Hres" with "H") as "[H|H]".
+  - iPoseProof ("Hp1" with "H") as "(%HNone & HH)".
+    destruct (p2 !! s) eqn:Heq.
+    * exfalso. pose proof (elem_of_disjoint (dom p1) (dom p2)) as [Hdis2 _].
+      destruct (p1 !! s) eqn:Heqq; try congruence.
+      eapply Hdis2; first done.
+      all: apply elem_of_dom; eexists; try done. 
+    * iSplitR.
+      -- iPureIntro. rewrite lookup_union_with. 
+         rewrite Heq. destruct (p1 !! s); cbn; congruence.
+      -- iApply (wp_link_execs with "[HT3 Hp2] [HH]"); last by iLeft. unfold can_link; repeat iSplit; (try by iPureIntro); done.
+  - iDestruct ("Hp2" with "H") as "(%HNone & HH)".
+    destruct (p1 !! s) eqn:Heq.
+    * exfalso. pose proof (elem_of_disjoint (dom p1) (dom p2)) as [Hdis2 _].
+      destruct (p2 !! s) eqn:Heqq; try congruence.
+      eapply Hdis2; first done.
+      all: apply elem_of_dom; eexists; try done. 
+    * iSplitR.
+      -- iPureIntro. rewrite lookup_union_with. 
+         rewrite Heq. destruct (p2 !! s); cbn; congruence.
+      -- iApply (wp_link_execs with "[HT3 Hp2] [HH]"); last by iRight. unfold can_link; repeat iSplit; (try by iPureIntro); done.
 Qed.
 
 
